theories/examples/scall.v
@@ -1,0 +1,109 @@
+From iris.algebra Require Import frac.
+From iris.proofmode Require Import tactics.
+Require Import Eqdep_dec List.
+From cap_machine Require Import rules logrel stack_macros. 
+
+Section scall.
+  Context `{memG Σ, regG Σ, STSG Σ, logrel_na_invs Σ,
+            MonRef: MonRefG (leibnizO _) CapR_rtc Σ,
+            Heap: heapG Σ}.
+
+  (* Macro for stack calling. Note that the prologue and epilogue does 
+     not include storing and loading private state on the stack. *)
+  
+  (* the prologue pushes the activation code, the old pc and stack points, 
+     sets up the return capability and adv stack capability, then jumps to adversary code *)
+  (* r1 is the register containg the adversary capability *)
+  Definition scall_prologue_instrs epilogue_off r1 :=
+    (* push activation code *)
+    push_z_instrs r_stk w_1 ++
+    push_z_instrs r_stk w_2 ++
+    push_z_instrs r_stk w_3 ++
+    push_z_instrs r_stk w_4a ++             
+    push_z_instrs r_stk w_4b ++
+    push_z_instrs r_stk w_4c ++
+    (* push old pc *)
+    [move_r r_t1 PC;
+    lea_z r_t1 epilogue_off;
+    lea_z r_stk 1; store_r r_stk r_t1; (* push_r r_t1 *)
+    (* push stack pointer *)
+    lea_z r_stk 1;
+    store_r r_stk r_stk;
+    (* set up protected return pointer *)
+    move_r r_t0 r_stk;
+    lea_z r_t0 (-7)%Z;
+    restrict_z r_t0 (local_e);
+    (* restrict stack capability *)
+    geta r_t1 r_stk;
+    add_r_z r_t1 r_t1 1;
+    gete r_t2 r_stk;
+    subseg_r_r r_stk r_t1 r_t2] ++
+    (* clear the unused part of the stack *)
+    (* mclear r_stk: *)
+    mclear_instrs r_stk 10 2 ++ (* 10 and 2 correspond to the offsets to iter in a contiguous mclear *)
+    rclear_instrs (list_difference all_registers [PC;r_stk;r_t0;r1]).
+
+  Definition scall_prologue (a : list Addr) p epilogue_off r1 :=
+    ([∗ list] a_i;w_i ∈ a;(scall_prologue_instrs epilogue_off r1), a_i ↦ₐ[p] w_i)%I.
+
+  Lemma scall_prologue_spec
+        (* adress arithmetic *) a_r_adv b_r_adv a_act a_cont a_next
+        (* scall parameters *) a a_first a_last p' epilogue_off r1
+        (* program counter *) p g b e
+        (* stack capability *) b_r e_r a_r
+        (* continuation *) φ :
+    isCorrectPC (inr ((p,g),b,e,a_first)) → isCorrectPC (inr ((p,g),b,e,a_last)) →
+    contiguous a →
+    a !! 0 = Some a_first -> list.last a = Some a_last ->
+    PermFlows p p' →
+
+    (a_r + 1)%a = Some a_act →
+    (a_r + 8)%a = Some a_r_adv →
+    (a_r + 9)%a = Some b_r_adv →
+    (a_first + (13 + epilogue_off))%a = Some a_cont →
+    (a_last + 1)%a = Some a_next →
+
+    (▷ scall_prologue a p' epilogue_off r1
+   ∗ ▷ PC ↦ᵣ inr ((p,g),b,e,a_first)
+   ∗ ▷ r_stk ↦ᵣ inr ((RWLX,Local),b_r,e_r,a_r)
+   ∗ ▷ (∃ wsr, [∗ list] r_i;w_i ∈ list_difference all_registers [PC;r_stk;r1]; wsr, r_i ↦ᵣ w_i)
+   ∗ ▷ (∃ ws_own, [[a_act, a_r_adv]]↦ₐ[RWLX][[ws_own]]) (* local stack *)
+   ∗ ▷ (∃ ws_adv, [[b_r_adv, e_r]]↦ₐ[RWLX][[ws_adv]]) (* adv stack *)
+   ∗ ▷ (PC ↦ᵣ inr (p,g,b,e,a_next)
+            ∗ r_stk ↦ᵣ inr ((RWLX,Local),b_r_adv,e_r,a_r_adv)
+            ∗ r_t0 ↦ᵣ inr ((E,Local),b_r,e_r,a_act)
+            ∗ ([∗ list] r_i ∈ list_difference all_registers [PC;r_stk;r_t0;r1], r_i ↦ᵣ inl 0%Z)
+            ∗ [[ a_act, a_r_adv ]]↦ₐ[RWLX][[ [inl w_1;
+                                             inl w_2;
+                                             inl w_3;
+                                             inl w_4a;
+                                             inl w_4b;
+                                             inl w_4c;
+                                             inr (p,g,b,e,a_cont);
+                                             inr (RWLX,Local,b_r,e_r,b_r_adv)] ]] (* local stack *)
+            ∗ [[ b_r_adv, e_r ]] ↦ₐ[RWLX] [[ region_addrs_zeroes b_r_adv e_r ]] (* cleared adv stack *)
+            ∗ scall_prologue a p' epilogue_off r1 -∗ 
+            WP Seq (Instr Executable) {{ φ }})
+   ⊢ WP Seq (Instr Executable) {{ φ }})%I. 
+  Proof.
+    iIntros (Hvpc1 Hvpc2 Ha Hfirst Hlast Hfl Hact Hadva Hadvb Hcont Hnext)
+            "(>Hscall & >HPC & >Hr_stk & >Hr1 & >Hgen_reg & >Hstack & Hφ)".
+    rewrite /scall_prologue.
+    iDestruct (big_sepL2_length with "Hscall") as %Hlength.
+    iDestruct (contiguous_program_split with "Hscall") as (a1 a2 a1_last a2_first) "(Hpush & Hprog & #Hcont)"; [auto|cbv;auto|..].
+    { rewrite app_length. apply PeanoNat.Nat.lt_lt_add_r. cbv. auto. } (* Make tactic for lengths *)
+    iDestruct "Hcont" as %(Ha1 & Ha2 & Happ & Ha1_last & Ha2_first). 
+    
+    
+    
+  Admitted.
+
+
+
+  Definition scall_epilogue_instrs :=
+    (* pop the restore code *)
+    (* to shorten the program we will do it all at once *)
+    [sub_z_z r_t1 0 7; lea_r r_stk r_t1]. 
+
+
+End scall. 
